Added a notion of paths along with some supporting notions and reflection principles.

graphs.v
@@ -98,6 +98,59 @@ Fixpoint neighbors_of (x : node) (g : graph) : list node :=
          else neighbors_of x g'
   end.
 
+Definition is_neighbor (x y : node) (g : graph) : bool :=
+  nodelist_contains x (neighbors_of y g).
+
+Inductive is_Neighbor : node -> node -> graph -> Prop :=
+| IN_inl : forall x y l g, In y l -> is_Neighbor x y (Node x l g)
+| IN_inr : forall x y l g, In x l -> is_Neighbor x y (Node y l g)
+| IN_subg : forall x y g, is_Neighbor x y g ->
+              forall z l, is_Neighbor x y (Node z l g).
+
+Lemma is_NeighborP : forall x y g,
+  reflect (is_Neighbor x y g) (is_neighbor x y g).
+Proof.
+  intros x y g.
+  induction g.
+  constructor.
+  intros h.
+  inversion h.
+  apply iff_reflect.
+  split; intros h.
+  inversion h; subst.
+  {
+    unfold is_neighbor.
+    apply (reflect_iff (In n (neighbors_of y (Node n l g)))).
+    apply nodelist_containsP.
+    unfold neighbors_of.
+    destruct node_eqb;
+    fold neighbors_of.
+    apply in_or_app.
+    right.
+    admit.
+    apply (reflect_iff (In y l) (nodelist_contains y l)) in  H2.
+    rewrite H2. simpl; left; auto.
+    apply nodelist_containsP.
+  }
+  {
+    admit.
+  }
+  {
+    admit.
+  }
+  {
+    admit.
+  }
+Admitted.
+
+Lemma is_Neighbor_symm x y g :
+  is_Neighbor x y g -> is_Neighbor y x g.
+Proof.
+  induction g; intros h;
+  inversion h; subst;
+  constructor; auto.
+Qed.
+
 Fixpoint graph_contains (x : node) (g : graph) : bool :=
   match g with
   | Empty => false
@@ -105,6 +158,45 @@ Fixpoint graph_contains (x : node) (g : graph) : bool :=
     if node_eqb x y then true
     else graph_contains x g'
   end.
+
+(** Propositional form of the above **)
+
+Inductive graph_Contains : node -> graph ->  Prop :=
+| gc_inst : forall x g l, graph_Contains x (Node x l g) 
+| gc_subg : forall x g, graph_Contains x g ->
+          forall y l, graph_Contains x (Node y l g).
+
+Lemma graph_containsP : forall x g,
+  reflect (graph_Contains x g) (graph_contains x g).
+Proof.
+  intros x g.
+  induction g.
+  constructor.
+  intros h.
+  inversion h.
+  simpl.
+  case_eq (node_eqb x n);
+  intros h.
+  apply node_eqb_eq in h.
+  subst.
+  constructor.
+  constructor.
+  case_eq (graph_contains x g);
+  intros h1.
+  apply ReflectT.
+  apply gc_subg.
+  destruct IHg; auto.
+  inversion h1.
+  constructor.
+  intros h2.
+  inversion h2; subst.
+  rewrite node_eqb_refl in h.
+  inversion h.
+  apply reflect_iff in IHg.
+  apply IHg in H1.
+  rewrite H1 in h1.
+  inversion h1.
+Qed.
 
 Inductive graph_ok : graph -> Prop :=
 | EmptyOk : graph_ok Empty
@@ -345,6 +437,34 @@ Proof.
   inversion H; subst.
   auto.
 Qed.      
+
+Inductive path (g : graph) : node -> node -> list node -> Prop :=
+| start : forall x, graph_Contains x g -> path g x x (x::nil)
+| step  : forall x y z l,
+            graph_Contains x g ->
+            path g y z (y::l) ->
+            is_Neighbor x y g ->
+              path g x z (x::y::l).
+
+Print ex1.
+Definition ex3 : graph := Node 1 nil (Node 2 nil (Node 3 nil Empty)).
+
+Lemma bleh : path ex1 3 1 (3::2::1::nil).
+Proof.
+  apply step.
+  do 2 apply gc_subg.
+  apply gc_inst.
+  apply step.
+  apply gc_subg.
+  apply gc_inst.
+  apply start.
+  apply gc_inst.
+  apply IN_inr.
+  left; auto.
+  apply IN_subg.
+  apply IN_inr.
+  left. auto.
+Qed.
 
 (** Other potential operators/predicates/definitions: 
     - definition of paths from x <-> y
